src/syntax/FStarC.Syntax.Embeddings.AppEmb.fsti
@@ -1,0 +1,22 @@
+module FStarC.Syntax.Embeddings.AppEmb
+
+open FStarC.Syntax.Syntax
+open FStarC.Syntax.Embeddings.Base
+
+type appemb 'a =
+  args -> option ('a & args)
+
+let (let?) o f = match o with | None -> None | Some v -> f v
+
+val (<*>) : appemb ('a -> 'b) -> appemb 'a -> appemb 'b
+val (<**>) : appemb ('a -> 'b) -> embedding 'a -> appemb 'b
+
+val pure (x : 'a) : appemb 'a
+
+val (<$>) : ('a -> 'b) -> appemb 'a -> appemb 'b
+
+val (<$$>) : ('a -> 'b) -> embedding 'a -> appemb 'b
+
+val run : args -> appemb 'a -> option 'a
+
+val wrap : (term -> option 'a) -> appemb 'a
